Factorial Refined

theories/Commons/RegisterBank.v
@@ -7,13 +7,13 @@ Definition reg := nat.
 (* [regmap] is a mapping from registers to a value *)
 Definition regbank : Type := gmap reg val.
 
-Definition get_reg (ρ: regbank) (r: reg) : val :=
+Definition regbank_get (ρ: regbank) (r: reg) : val :=
   match ρ !! r with
   | Some v => v
   | None => 0%Z (* Default val *)
   end.
 
-Definition set_reg (ρ: regbank) (r: reg) (v: val) : regbank :=
+Definition regbank_set (ρ: regbank) (r: reg) (v: val) : regbank :=
   <[r := v]>ρ.
 
 (** ** Logical Connectives  *)
@@ -22,10 +22,10 @@ Class LogicRegisterAssert (R V : Type) :=
   regbank_assert : regbank -> R -> V -> Prop.
 
 Instance regbank_assert_single : LogicRegisterAssert reg val :=
-  fun ρ key val => get_reg ρ key = val.
+  fun ρ key val => regbank_get ρ key = val.
 
 Instance regbank_assert_list : LogicRegisterAssert (list reg) (list val) :=
-  fun ρ keys vals => map (get_reg ρ) keys = vals.
+  fun ρ keys vals => map (regbank_get ρ) keys = vals.
 
 Notation "ρ @ r '⇒' v" :=
   (regbank_assert ρ r%nat v%Z)
@@ -39,8 +39,19 @@ Notation "ρ1 @ r1 '<=>' ρ2 @ r2" :=
     (at level 60, ρ2 at next level, no associativity).
 
 Notation "'⟦' r '⇐' v '⟧' ρ" :=
-  (set_reg ρ r%nat v%Z)
+  (regbank_set ρ r%nat v%Z)
     (at level 20, ρ at level 20, right associativity).
+
+Create HintDb regbank discriminated.
+
+Hint Unfold
+  regbank
+  regbank_get
+  regbank_set
+  regbank_assert
+  regbank_assert_single
+  regbank_assert_list
+  regbank_same : regbank.
 
 Lemma regbank_assert_unfold ρ :
   ∀ r v tl tv,
@@ -48,38 +59,51 @@ Lemma regbank_assert_unfold ρ :
   ρ @ tl ⇒ tv ->
   ρ @ (r :: tl) ⇒ (v :: tv).
 Proof.
-  intros r v tl tv.
-  unfold regbank_assert, regbank_assert_single, regbank_assert_list.
-  intros Hv Htl. simpl.
-  f_equal.
-  - assumption.
-  - eassumption.
+  autounfold with regbank.
+  intros r v tl tv Hv Htl.
+  simpl. now f_equal.
 Qed.
 
 Lemma regbank_assert_nil ρ :
   ρ @ [] ⇒ [].
-Proof. now unfold regbank_assert, regbank_assert_list. Qed.
+Proof. now autounfold with regbank. Qed.
 
 Lemma regbank_set_discard ρ :
-  ∀ r1 r2 v1 v2,
+  ∀ (r1 r2 : reg) v1 v2,
   r2 ≠ r1 ->
   ρ @ r1 ⇒ v1 ->
   ⟦r2 ⇐ v2⟧ρ @ r1 ⇒ v1.
 Proof.
-  intros r1 r2 v1 v2 Hneq.
-  unfold regbank_assert, regbank_assert_single, set_reg, get_reg.
-  intros Hr.
-  unfold regbank in *.
+  autounfold with regbank.
+  intros r1 r2 v1 v2 Hneq Hr.
   now rewrite lookup_insert_ne.
+Qed.
+
+Lemma regbank_set_discard_list :
+  ∀ regs args r ρ v,
+  r ∉ regs ->
+  ρ @ regs ⇒ args ->
+  ⟦r ⇐ v⟧ρ @ regs ⇒ args.
+Proof using Type.
+  autounfold with regbank.
+  intros regs args r ρ v Hr Hmap.
+  induction args as [| a args IH ] in regs, Hmap, Hr |- *.
+  - apply map_eq_nil in Hmap. now subst regs.
+  - apply map_eq_cons in Hmap.
+    destruct Hmap as (reg & tl & -> & Hreg & Hmap).
+    apply not_elem_of_cons in Hr.
+    destruct Hr as [Hr Htl].
+    simpl. f_equal.
+    + now rewrite (lookup_insert_ne ρ).
+    + now apply IH.
 Qed.
 
 Lemma regbank_set_use ρ :
   ∀ r v,
   ⟦r ⇐ v⟧ρ @ r ⇒ v.
 Proof.
+  autounfold with regbank.
   intros r v.
-  unfold regbank_assert, regbank_assert_single, set_reg, get_reg.
-  unfold regbank in *.
   now rewrite lookup_insert_eq.
 Qed.
 
@@ -87,7 +111,62 @@ Lemma regbank_never_empty ρ:
   ∀ r : reg,
   ∃ v, ρ @ r ⇒ v.
 Proof.
+  autounfold with regbank.
   intros r.
-  unfold regbank_assert, regbank_assert_single, get_reg.
   destruct (ρ !! r); now eexists.
 Qed.
+
+Lemma regbank_simpl_inj ρ:
+  ∀ (r: reg) v1 v2,
+  ρ @ r ⇒ v1 ->
+  ρ @ r ⇒ v2 ->
+  v1 = v2.
+Proof.
+  autounfold with regbank in *.
+  intros r v1 v2 <- ->.
+  easy.
+Qed.
+
+Lemma regbank_list_inj ρ:
+  ∀ (r: list reg) v1 v2,
+  ρ @ r ⇒ v1 ->
+  ρ @ r ⇒ v2 ->
+  v1 = v2.
+Proof.
+  autounfold with regbank in *.
+  intros r v1 v2 <- ->.
+  easy.
+Qed.
+
+Lemma regbank_list_length ρ:
+  ∀ (regs: list reg) vals,
+  ρ @ regs ⇒ vals ->
+  length vals = length regs.
+Proof.
+  autounfold with regbank in *.
+  intros regs vals <-.
+  now apply length_map.
+Qed.
+
+Ltac simpl_regs tac :=
+  match goal with
+  | [ |- ?ρ @ [] ⇒ _ ] =>
+      apply regbank_assert_nil
+  | [ H: ?ρ @ ?r ⇒ ?v |- ?ρ @ ?r ⇒ _ ] =>
+      exact H
+  | [ |- ⟦?r ⇐ _⟧?ρ @ ?r ⇒ _ ] =>
+      apply regbank_set_use
+  | [ |- ⟦_ ⇐ _⟧?ρ @ ?r ⇒ _ ] =>
+      apply regbank_set_discard; [tac| simpl_regs tac]
+  | [ |- ?ρ @ (?r :: ?tl) ⇒ _ ] =>
+      apply regbank_assert_unfold; simpl_regs tac
+  | [ H1: ?ρ @ ?r ⇒ ?v1, H2: ?ρ @ ?r ⇒ ?v2 |- _ ] =>
+      let Heq := fresh "Heq" in
+      assert (Heq: v2 = v1) by
+        (apply (regbank_simpl_inj _ _ _ _ H2 H1)
+         || apply (regbank_list_inj _ _ _ _ H2 H1));
+      simplify_eq;
+      clear H2; try (simpl_regs tac)
+  end.
+
+Global Tactic Notation "simregs" := simpl_regs lia.
