theories/Prelude/Memory.v
@@ -6,7 +6,7 @@ Definition val : Type := Z.
 Definition loc : Type := positive.
 
 (* [memory] is a mapping from location to a value *)
-Abbreviation memory := (gmap loc val).
+Definition memory := (gmap loc val).
 
 Definition loc_to_val (l: loc) : val := Zpos l.
 
@@ -17,69 +17,16 @@ Definition val_to_loc (v: val) : option loc :=
 
 Definition get_at (addr: val) (m: memory) : option val :=
   match val_to_loc addr with
-  | Some loc => m !! loc
+  | Some l => m !! l
   | None => None
   end.
 
-Definition update_at (addr: val) (f: val -> val) (m: memory) : option memory
-  := match val_to_loc addr with
-     | Some loc => Some (alter f loc m)
-     | None => None
-     end.
-
 Definition set_at (addr: val) (v: val) (m: memory) : option memory :=
-  update_at addr (fun _ => v) m.
-
-Lemma get_at_unfold : ∀ addr m v,
-  get_at addr m = Some v ->
-  ∃ l, val_to_loc addr = Some l ∧ m !! l = Some v.
-Proof using Type.
-  intros addr m v H.
-  unfold get_at in H.
-  case_match; try congruence.
-  eexists. split; eassumption || reflexivity.
-Qed.
-
-Lemma update_at_unfold : ∀ addr f m m',
-  update_at addr f m = Some m' ->
-  ∃ loc,
-    val_to_loc addr = Some loc ∧
-    alter f loc m = m'.
-Proof using Type.
-  intros addr f m m' H.
-  unfold update_at in H.
-  case_match eqn:Hloc; try congruence.
-  eexists. split.
-  - reflexivity.
-  - now inv H.
-Qed.
-
-Lemma alter_union_left f loc (m1 m2: memory) :
-  m1 ##ₘ m2 ->
-  m2 !! loc = None ->
-  alter f loc (m1 ∪ m2) = alter f loc m1 ∪ m2.
-Proof using Type.
-  intros Hdij Hnin.
-  unfold union, map_union.
-  rewrite (alter_union_with_l _ _ m1).
-  - reflexivity.
-  - intros x y H1 H2. exfalso.
-    rewrite map_disjoint_alt in Hdij.
-    destruct (Hdij loc) as [? | ?]; congruence.
-  - intros x H1 H2. congruence.
-Qed.
-
-Lemma alter_union_right f loc (m1 m2: memory) :
-  m1 ##ₘ m2 ->
-  m1 !! loc = None ->
-  alter f loc (m1 ∪ m2) = m1 ∪ alter f loc m2.
-Proof using Type.
-  intros Hdij Hnin.
-  unfold union, map_union.
-  rewrite (alter_union_with_r _ _ m1).
-  - reflexivity.
-  - intros x y H1 H2. exfalso.
-    rewrite map_disjoint_alt in Hdij.
-    destruct (Hdij loc) as [? | ?]; congruence.
-  - intros x H1 H2. congruence.
-Qed.
+  match val_to_loc addr with
+  | Some l =>
+      match m !! l with
+      | None => None
+      | Some _ => Some (alter (fun _ => v) l m)
+      end
+  | None => None
+  end.
