theories/RTL/WP.v
@@ -13,85 +13,98 @@ Section RTLWP.
   Let Λ : lang := rtl_lang.
   Context (P: prog Λ).
 
-  Definition wp (Q: postcondition) f pc : logic :=
-    fun ρ m n => safe P (uncurry Q) ([], State f pc ρ, m) n.
+  Implicit Types Q : postcondition.
 
-  Lemma wp_ret (Q: postcondition) f pc : ∀ r v,
-    f@pc is <<{ ret r }>> ->
-    ⊢ ▷ (r ⇒ v ∧ ⌜Q v⌝ₘ) -> wp Q f pc.
+  Definition wp ρ f pc Q : logic :=
+    fun n m => safe P (uncurry Q) ([], State f pc ρ, m) n.
+
+  Lemma wp_ret ρ f pc Q :
+    ∀ r v,
+    f @ pc is <<{ ret r }>> ->
+    ρ @ r ⇒ v ->
+    ▷⌜Q v⌝ₘ ⊩ wp ρ f pc Q.
   Proof using Type.
-    intros r v Hpc ρ m [] H; [apply safe_init | ].
-    unfold_Prop. destruct H as [Hv HQ]. subst.
+    intros r v Hpc Hv.
+    intros [] m Hwp; [apply safe_init | unfold_Prop].
     apply safe_to_step.
-    - eexists; econstructor; now eauto.
-    - intros t Hstep. inv Hstep. apply final_is_safe. econstructor.
+    - do 2 econstructor; eassumption || reflexivity.
+    - intros t Hstep. inv Hstep. simregs.
+      apply final_is_safe. econstructor.
       split.
       + reflexivity.
       + now unfold uncurry.
   Qed.
 
-  Lemma wp_nop Q f pc : ∀ pc',
-    f@pc is <<{ nop -> pc' }>> ->
-    ⊢ (▷ wp Q f pc') -> wp Q f pc.
+  Lemma wp_nop ρ f pc Q :
+    ∀ pc',
+    f @ pc is <<{ nop -> pc' }>> ->
+    ▷wp ρ f pc' Q ⊩ wp ρ f pc Q.
   Proof using Type.
-    intros v Hpc ρ m [] Hwp; [apply safe_init | ].
+    intros v Hpc.
+    intros [] m Hwp; [apply safe_init | unfold_Prop].
     apply safe_to_step.
-    - repeat econstructor; now eauto.
-    - intros ? Hs. now inv Hs.
+    - do 2 econstructor; eassumption || reflexivity.
+    - intros ? Hs.
+      now inv Hs.
   Qed.
 
-  Lemma wp_op Q f pc : ∀ dst op args pc' vals v,
-    f@pc is <<{ dst := @op args -> pc' }>> ->
-    ⊢ (args ⇒ vals ∧
-       ⌜eval_op op vals = Some v⌝ ∧
-       ▷ ⟦dst ⇐ v⟧wp Q f pc') ->
-    wp Q f pc.
+  Lemma wp_op ρ f pc Q :
+    ∀ dst op args pc' vals v,
+    f @ pc is <<{ dst := @op args -> pc' }>> ->
+    ρ @ args ⇒ vals ->
+    eval_op op vals = Some v ->
+    ▷wp (⟦dst ⇐ v⟧ρ) f pc' Q ⊩ wp ρ f pc Q.
   Proof using Type.
-    intros dst op args pc' vals v Hpc ρ m [] (Hargs & Hv & Hwp);
-      [apply safe_init | ]. unfold_Prop. subst.
+    intros dst op args pc' vals v Hpc Hvals Hv.
+    intros [] m Hwp; [apply safe_init | unfold_Prop].
     apply safe_to_step.
-    - repeat econstructor; now eauto.
-    - intros ? Hs. now inv Hs.
+    - do 2 econstructor; eassumption || reflexivity.
+    - intros ? Hs. inv Hs.
+      now simregs.
   Qed.
 
-  Lemma wp_load Q f pc : ∀ dst src pc' addr v,
-    f@pc is <<{ dst := !src -> pc' }>> ->
-    ⊢ (src ⇒ addr ∧ addr ↦ v ∧ ▷ ⟦dst ⇐ v⟧ wp Q f pc') ->
-    wp Q f pc.
+  Lemma wp_load ρ f pc Q :
+    ∀ dst src pc' addr v,
+    f @ pc is <<{ dst := !src -> pc' }>> ->
+    ρ @ src ⇒ addr ->
+    (addr ↦ v ∧ ▷ wp (⟦dst ⇐ v⟧ρ) f pc' Q) ⊩ wp ρ f pc Q.
   Proof using Type.
-    intros dst src pc' addr v Hpc ρ m [] (Haddr & Hmem & Hwp)
-    ; [apply safe_init | ]. unfold_Prop. subst.
+    intros dst src pc' addr v Hpc Haddr.
+    intros [] m (Hmem & Hwp); [apply safe_init | unfold_Prop].
     apply safe_to_step.
-    - repeat econstructor; now eauto.
-    - intros ? Hs. now inv Hs.
+    - do 2 econstructor; eassumption || reflexivity.
+    - intros ? Hs. inv Hs.
+      now simregs.
   Qed.
 
-  Lemma wp_store Q f pc : ∀ dst src pc' addr v,
-    f@pc is <<{ !dst := src -> pc' }>> ->
-    ⊢ (dst ⇒ addr ∧
-       src ⇒ v ∧
-       ▷ ⟦addr <- v⟧ wp Q f pc') ->
-    wp Q f pc.
+  Lemma wp_store ρ f pc Q :
+    ∀ dst src pc' addr v,
+    f @ pc is <<{ !dst := src -> pc' }>> ->
+    ρ @ dst ⇒ addr ->
+    ρ @ src ⇒ v ->
+    ▷⟦addr <- v⟧ wp ρ f pc' Q ⊩ wp ρ f pc Q.
   Proof using Type.
-    intros dst src pc' addr v H ρ m [] (Haddr & Hmem & Hwp);
-      [apply safe_init | ]. unfold_Prop. subst.
+    intros dst src pc' addr v H Haddre Hmem.
+    intros [] m Hwp; [apply safe_init | unfold_Prop].
     destruct Hwp as (m' & Hm' & Hwp). apply safe_to_step.
-    - repeat econstructor; now eauto.
-    - intros ? Hs. now inv Hs.
+    - do 2 econstructor; eassumption || reflexivity.
+    - intros ? Hs. inv Hs.
+      now simregs.
   Qed.
 
-  Lemma wp_cond Q f pc : ∀ cond ifso ifnot v,
-    f@pc is <<{ if cond then goto ifso else goto ifnot }>> ->
-    ⊢ (cond ⇒ v ∧
-       if (v =? 0)%Z
-       then ▷ wp Q f ifso
-       else ▷ wp Q f ifnot) ->
-    wp Q f pc.
+  Lemma wp_cond ρ f pc Q :
+    ∀ cond ifso ifnot v pc',
+    f @ pc is <<{ if cond then goto ifso else goto ifnot }>> ->
+    ρ @ cond ⇒ v ->
+    (if (v =? 0)%Z then ifso else ifnot) = pc' ->
+    ▷wp ρ f pc' Q ⊩ wp ρ f pc Q.
   Proof using Type.
-    intros cond ifso ifnot v H ρ m [] (Hv & Hwp); [apply safe_init | ].
-    unfold_Prop. apply safe_to_step.
-    - repeat econstructor; now eauto.
-    - intros ? Hs. inv Hs. now destruct (get_reg ρ cond =? 0)%Z.
+    intros cond ifso ifnot v pc' H Hcond Hpc.
+    intros [] m Hwp; [apply safe_init | unfold_Prop].
+    apply safe_to_step.
+    - do 2 econstructor; eassumption || reflexivity.
+    - intros ? Hs. inv Hs.
+      now simregs.
   Qed.
 
   Definition hoare (Pre: precondition) f (Post: postcondition) : Prop :=
@@ -118,22 +131,21 @@ Section RTLWP.
     - lia.
   Qed.
 
-  Lemma wp_call f pc Q : ∀ dst name args pc' vals fn Pre Post,
-    f@pc is <<{ dst := @call name args -> pc' }>> ->
-    ⊢ (args ⇒ vals ∧
-       ⌜find_fun P name = Some fn⌝ ∧
-       ⌜length (fn_regs fn) = length args⌝ ∧
-       ⌜hoare Pre fn Post⌝ ∧
-       ⌜Pre vals⌝ₘ ∧
-       ▷ (∀ v, ⊢ₘ ⌜Post v⌝ₘ -> ⟦dst ⇐ v⟧ wp Q f pc')) ->
-    wp Q f pc.
+  Lemma wp_call ρ f pc Q :
+    ∀ dst name args pc' vals fn Pre Post,
+    f @ pc is <<{ dst := @call name args -> pc' }>> ->
+    ρ @ args ⇒ vals ->
+    find_fun P name = Some fn ->
+    length (fn_regs fn) = length args ->
+    hoare Pre fn Post ->
+    (⌜Pre vals⌝ₘ ∧ ▷(∀ v, ⌜Post v⌝ₘ ⊩ₘ wp (⟦dst ⇐ v⟧ρ) f pc' Q)) ⊩
+    wp ρ f pc Q.
   Proof using Type.
-    intros dst sig args pc' vals fn Pre Post H ρ m [ | n]
-      (Hargs & Hfun & Hlen & Hspec & Hpre & Hwp); [apply safe_init | ].
-    unfold_Prop. subst.
+    intros dst sig args pc' vals fn Pre Post H Hargs Hfun Hlen Hspec.
+    intros [|n] m (Hpre & Hwp); [apply safe_init | unfold_Prop ].
     apply safe_to_step.
-    - repeat econstructor; now eauto.
-    - intros t Hs. inv Hs.
+    - do 2 econstructor; eassumption || reflexivity.
+    - intros t Hs. inv Hs. simregs.
       apply safe_from_progress.
       intros [[σ' s] m''] n' Hn Hsteps.
       apply unfold_call in Hsteps.
@@ -145,7 +157,9 @@ Section RTLWP.
           apply ret_not_stuck.
         * subst. now apply lift_not_stuck.
         * apply Hspec with (n := n+1); auto.
-          now rewrite length_map.
+          rewrite Hlen.
+          eapply regbank_list_length.
+          eassumption.
         * lia.
       + eapply safe_implies_progress in Hrest.
         * eassumption.
@@ -154,52 +168,37 @@ Section RTLWP.
         * lia.
   Qed.
 
-  Local Lemma get_regs_not_in : ∀ regs args r ρ v,
-    r ∉ regs ->
-    map (get_reg ρ) regs = args ->
-    map (get_reg (<[r:=v]> ρ)) regs = args.
-  Proof using Type.
-    intros regs args r ρ v Hr Hmap.
-    induction args as [| a args IH ] in regs, Hmap, Hr |- *.
-    - apply map_eq_nil in Hmap. now subst regs.
-    - apply map_eq_cons in Hmap.
-      destruct Hmap as (reg & tl & -> & Hreg & Hmap).
-      apply not_elem_of_cons in Hr.
-      destruct Hr as [Hr Htl].
-      simpl. f_equal.
-      + unfold get_reg. now rewrite (fin_maps.lookup_insert_ne ρ).
-      + now apply IH.
-  Qed.
-
   Local Lemma initial_context_exists : ∀ args regs,
     length args = length regs ->
     NoDup regs ->
-    ∃ ρ, map (get_reg ρ) regs = args.
+    ∃ ρ, ρ @ regs ⇒ args.
   Proof using Type.
     intros args.
     induction args as [| v args IH]; intros regs Hlen Hdup.
-    - exists ∅. symmetry in Hlen. now rewrite (nil_length_inv _ Hlen).
+    - exists ∅. symmetry in Hlen. rewrite (nil_length_inv _ Hlen).
+      simregs.
     - simpl in Hlen. destruct regs as [| r regs]; inv Hlen as [ H ].
       apply NoDup_cons in Hdup.
       destruct Hdup as [Hr Hdup].
       destruct (IH _ H Hdup) as [ρ Hmap].
-      exists (<[r := v]>ρ).
-      simpl. f_equal.
-      + unfold get_reg. now rewrite (fin_maps.lookup_insert_eq ρ).
-      + now apply get_regs_not_in.
+      exists (⟦r ⇐ v⟧ρ).
+      apply regbank_assert_unfold.
+      + simregs.
+      + now apply regbank_set_discard_list.
   Qed.
 
   Lemma hoare_from_wp (Pre: precondition) f (Post: postcondition):
-    (∀ args,
-       ⊢ (⌜Pre args⌝ₘ ∧ fn_regs f ⇒ args) -> wp Post f (fn_entrypoint f))
+    (∀ ρ args,
+       ρ @ (fn_regs f) ⇒ args ->
+       ⌜Pre args⌝ₘ ⊩ wp ρ f (fn_entrypoint f) Post)
     -> hoare Pre f Post.
   Proof using Type.
-    intros H args m [ ] Hlen Hpre; [apply safe_init | ].
-    unfold_Prop.
+    intros H args m [ ] Hlen Hpre; [apply safe_init | unfold_Prop ].
     apply safe_to_step.
     - destruct (initial_context_exists _ _ Hlen) as [ρ Hρ].
       + apply is_no_dup_sound. now apply fn_regs_no_dup.
       + do 2 econstructor; eassumption.
-    - intros ? Hs. inv Hs. eapply H. split; eassumption || reflexivity.
+    - intros ? Hs. inv Hs.
+      eapply H; eassumption || reflexivity.
   Qed.
 End RTLWP.
