theories/Playground/SimTest.v
@@ -1,0 +1,239 @@
+From RSL Require Import RelLogic Prelude.
+
+From stdpp Require Import strings.
+From stdpp Require Import gmap.
+From stdpp Require Import tactics.
+
+From RSL Require Import Simulations.FreeSim.
+From RSL Require Import Simulations.FreeSimRules.
+
+From RSL Require Import RTL.RTL.
+From RSL Require Import RTL.Notations.
+From RSL Require Import RTL.Semantics.
+
+From RSL Require Import RTL.SimRules.
+From RSL Require Import RTL.TargetRules.
+From RSL Require Import RTL.SourceRules.
+
+Import RTLNotations.
+
+Section T.
+  Let Λₜ : lang := rtl_lang.
+  Let Λₛ : lang := rtl_lang.
+  Context (Pₜ : prog Λₜ) (Pₛ : prog Λₛ).
+
+  Abbreviation fsim := (fsim WfNat WfNat Pₜ Pₛ).
+
+  Let reg_n : reg := 1.
+  Let reg_res : reg := 2.
+  Let reg_one : reg := 3.
+  Let reg_addr : reg := 4.
+
+  Definition fact_bad : function :=
+    {|
+      fn_name := "fact"%string;
+      fn_regs := [reg_n; reg_addr];
+      fn_entrypoint := 0;
+      fn_code :=
+        <<{{
+              0: reg_res := #1 -> 1;
+              1: !reg_addr := reg_res -> 2;
+              2: if reg_n then goto 6 else goto 3;
+              3: reg_res := reg_res * reg_n -> 4;
+              4: reg_one := !reg_addr -> 5;
+              5: reg_n := reg_n - reg_one -> 2;
+              6: ret reg_res;
+          }}>>;
+      fn_regs_no_dup := eq_refl;
+    |}.
+
+  Definition fact_good : function :=
+    {|
+      fn_name := "fact"%string;
+      fn_regs := [reg_n; reg_addr];
+      fn_entrypoint := 0;
+      fn_code :=
+        <<{{
+              0: reg_res := #1 -> 1;
+              1: !reg_addr := reg_res -> 2;
+              2: reg_one := #1 -> 3;
+              3: if reg_n then goto 6 else goto 4;
+              4: reg_res := reg_res * reg_n -> 5;
+              5: reg_n := reg_n - reg_one -> 3;
+              6: ret reg_res;
+        }}>>;
+      fn_regs_no_dup := eq_refl;
+    |}.
+
+  Notation
+    "'[' C ']' ρ '⊢' ft '@' pct  '<{' j ',' i '}=' fs '@' pcs '{{' Q '}}'" :=
+    (sim Pₜ Pₛ C ρ ft pct j i fs pcs Q%rlogic)
+      (at level 0, ft at level 0, fs at level 0, no associativity).
+
+  Notation
+    "'[' C ']' ρ '⊢' '{{' P '}}' ft '@' pct  '<{' j ',' i '}=' fs '@' pcs '{{' Q '}}'" :=
+    (hoare Pₜ Pₛ C ρ P%rlogic ft pct j i fs pcs Q%rlogic)
+      (at level 0, ft at level 0, fs at level 0, no associativity).
+
+  Lemma inv_proof ρₜ ρₛ P : ∀ l v,
+    [fsim] (ρₜ, ρₛ) ⊢
+    {{ (fun ρₜ ρₛ =>
+          ⌜∀ r, ~In r [reg_one; reg_addr] -> ρₜ @ r <=> ρₛ @ r⌝ ∗
+          ⌜ρₜ @ reg_one ⇒ v⌝ ∗
+          ⌜ρₛ @ reg_addr ⇒ l⌝ ∗
+          l →ₛ v ∗ P
+       ) ρₜ ρₛ
+    }}
+      fact_good @ 3 <{0, 0}= fact_bad @ 2
+    {{ fun vₜ vₛ =>
+         ⌜vₜ = vₛ⌝ ∗
+         l →ₛ v ∗
+         P
+    }}.
+  Proof using Type.
+    intros l v.
+    apply coind.
+    clear.
+    intros R ρₜ ρₛ CIH.
+    apply ipure. intros Hsame.
+    apply ipure. intros Hone.
+    apply ipure. intros Haddr.
+
+    destruct (Hsame reg_n) as (n & Htn & Hsn). 1: (cbv; lia).
+    destruct (Hsame reg_res) as (r & Htr & Hsr).  1: (cbv; lia).
+
+    eapply source_if; [ reflexivity | simregs | reflexivity |].
+    eapply target_if; [ reflexivity | simregs | reflexivity |].
+
+    destruct (n =? 0)%Z.
+    {
+      intros ? ? Hemp Ψ mtPre msPre ? ? Hpre mtPost msPost ? ? Hpost.
+
+      destruct Hpre as (mtv & msv & mtP & msP & ? & ? & ? & ? & Hs & HP).
+      destruct Hs as (Ht & (l' & Hl & Hs)).
+      destruct Hemp as (-> & ->).
+
+      eapply both_ret.
+      - reflexivity.
+      - reflexivity.
+      - simregs.
+      - simregs.
+      - rewrite (map_union_comm mtPost) by solve_map_disjoint.
+        rewrite (map_union_comm msPost) by solve_map_disjoint.
+        apply Hpost; try solve_map_disjoint.
+        eexists ∅, ∅, mtP, (msv ∪ msP). repeat split.
+        + solve_map_disjoint.
+        + solve_map_disjoint.
+        + subst. now rewrite !map_union_empty, !map_empty_union.
+        + subst. now rewrite !map_union_empty, !map_empty_union.
+        + exists ∅, msv, mtP, msP. repeat split.
+          * solve_map_disjoint.
+          * solve_map_disjoint.
+          * apply map_empty_union.
+          * now exists l'.
+          * assumption.
+    }
+    eapply source_op; [ reflexivity | simregs | simpl eval_op; intros ? Hv; inv Hv ].
+
+    eapply target_op; [ reflexivity | simregs | reflexivity | ].
+    eapply target_op; [ reflexivity | simregs | reflexivity | ].
+
+    eapply source_load; [reflexivity | simregs | ].
+    eapply source_op; [ reflexivity | simregs | simpl eval_op; intros ? Hv; inv Hv ].
+
+    eapply consequence.
+    3:{ apply CIH; lia. }
+    - intros mt ms H.
+      apply sep_pure_left.
+      {
+        intros r' Hr.
+        destruct (Hsame r' Hr) as (? & ? & ?).
+        rewrite !not_in_cons in Hr.
+        destruct Hr as (? & ? & _).
+
+        destruct (in_dec Nat.eq_dec r' [reg_n; reg_res])
+          as [[<- | [<- | ?]] | Hr].
+        - eexists. split; simregs.
+        - eexists. split; simregs.
+        - contradiction.
+        - rewrite !not_in_cons in Hr.
+          destruct Hr as (? & ? & _).
+          eexists. split; simregs.
+      }
+      apply sep_pure_left.
+      { simregs. }
+      apply sep_pure_left.
+      { simregs. }
+      easy.
+    - now simpl.
+  Qed.
+
+  Lemma fact_same ρₜ ρₛ:
+    ∀ addr,
+
+    (∀ r, ρₜ @ r <=> ρₛ @ r) ->
+    ρₛ @ reg_addr ⇒ addr ->
+
+    [fsim] (ρₜ, ρₛ) ⊢
+    {{
+        addr ₛ~ₜ addr
+    }}
+      fact_good @ 0 <{0, 0}= fact_bad @ 0
+    {{ fun vₜ vₛ =>
+         ⌜vₜ = vₛ⌝ ∗
+         addr ₛ~ₜ addr
+    }}.
+  Proof using Type.
+    intros addr Hsame Haddrs'.
+    eapply iex. intros v.
+
+    eapply source_op; [ reflexivity | simregs | intros ? Hv; inv Hv ].
+    eapply target_op; [ reflexivity | simregs | reflexivity | ].
+
+    destruct (Hsame reg_addr) as (? & Haddrs & Haddrt). simregs.
+
+    eapply consequence.
+    { apply sep_comm. }
+    { intros. apply entails_refl. }
+
+    eapply source_store; [ reflexivity | simregs | simregs | ].
+
+    eapply consequence.
+    { apply sep_comm. }
+    { intros. apply entails_refl. }
+
+    eapply target_store; [ reflexivity | simregs | simregs | ].
+    eapply target_op; [ reflexivity | simregs | reflexivity | ].
+
+    eapply consequence.
+    3: eapply fsim_mono; try apply inv_proof; lia.
+    - intros mt ms H.
+      apply sep_pure_left.
+      {
+        intros r Hr.
+        rewrite !not_in_cons in Hr.
+        destruct Hr as (? & ? & _).
+
+        destruct (in_dec Nat.eq_dec r [reg_res])
+          as [[-> | ?] | Hr].
+        - eexists. split; simregs.
+        - contradiction.
+        - rewrite !not_in_cons in Hr.
+          destruct Hr as (? & _).
+          destruct (Hsame r) as (? & ? & ?).
+          eexists. split; simregs.
+      }
+      apply sep_pure_left. 1: simregs.
+      apply sep_pure_left. 1: simregs.
+      apply sep_comm. apply H.
+    - intros vₜ vₛ. simpl.
+      eapply entails_frame_l.
+      intros mt ms H. eexists.
+      apply sep_comm. apply H.
+  Qed.
+
+End T.
+
+(* Memcopy avec déroulage de boucle ? *)
+(* Optimisations des nop ? *)
+(* Inlining à la main ? *)
