theories/Playground/ToyTest.v
@@ -1,0 +1,58 @@
+From RSL Require Import Prelude.
+
+From stdpp Require Import prelude strings fin_maps sorting.
+
+From RSL Require Import Toy.Toy.
+From RSL Require Import Toy.Notations.
+From RSL Require Import Toy.Compile.
+
+From RSL Require Import RTL.RTL.
+From RSL Require Import RTL.Notations.
+From RSL Require Import RTL.Simpl.
+
+Import ToyNotations.
+Import RTLNotations.
+
+Section Playground.
+  Let n : reg := 1.
+  Let result : reg := 2.
+  Let one : reg := 3.
+
+  Definition factorial_program : tfunction :=
+    {|
+      tfn_name := "fact"%string;
+      tfn_regs := [n];
+      tfn_code :=
+        <{|
+            result := #1;
+            one := #1;
+            while n {
+                result := result * n;
+                n := n - one
+            };
+            return result
+          |}>;
+      tfn_regs_no_dup := eq_refl;
+    |}.
+
+  Definition sortp (a b: node * instr) : Prop :=
+    match b, a with
+    | (x, _), (y, _) => x <= y
+    end.
+
+  (* Definition compile_and_opt (p: tfunction) : option function := *)
+  (*   match compile p with *)
+  (*   | Some c => Some $ remove_dead_code $ remove_nops c *)
+  (*   | None => None *)
+  (*   end. *)
+
+  (* Definition pp (p: option function) : list (node * instr) := *)
+  (*   match p with *)
+  (*   | Some m => merge_sort sortp $ map_to_list $ fn_code m *)
+  (*   | None => [] *)
+  (*   end. *)
+
+  (* Compute pp $ compile factorial_program. *)
+
+  (* Compute pp $ compile_and_opt factorial_program. *)
+End Playground.
