theories/Playground/WPTest.v
@@ -1,0 +1,115 @@
+From RSL Require Import Prelude.
+
+From stdpp Require Import strings.
+
+From RSL Require Import Commons.WP.
+From RSL Require Import Commons.Logic.
+
+From RSL Require Import RTL.RTL.
+From RSL Require Import RTL.Semantics.
+From RSL Require Import RTL.Notations.
+From RSL Require Import RTL.WP.
+
+Import RTLNotations.
+
+Section Play.
+  Let Λ : lang := rtl_lang.
+  Context (P: prog Λ).
+
+  Let x : reg := 0.
+  Let one : reg := 1.
+  Let ten : reg := 2.
+  Let diff : reg := 3.
+
+  Definition NodeInv f pc Q (NI : regbank -> logic) : Prop :=
+    ⌜⌝ ⊩ ∀ ρ, NI ρ -> wp P ρ f pc Q.
+
+  Definition test : function :=
+    {|
+      fn_name := "test"%string;
+      fn_regs := [];
+      fn_entrypoint := 0;
+      fn_code := <<{{
+            0: x := #0 -> 1;
+            1: one := #1 -> 2;
+            2: ten := #10 -> 3;
+            3: diff := ten - x -> 4;
+            4: if diff then goto 6 else goto 5;
+            5: x := x + one -> 3;
+            6: ret x;
+        }}>>;
+      fn_regs_no_dup := eq_refl;
+    |}.
+
+
+  Ltac step_acc Hpc :=
+    lazymatch type of Hpc with
+    | _ @ _ is Iop _ _ _ _ =>
+        eapply wp_op; [exact Hpc | simregs | reflexivity | ]
+
+    | _ @ _ is Icond _ _ _ =>
+        eapply wp_cond; [exact Hpc | simregs | reflexivity | ]
+
+    | _ @ _ is Ireturn _ =>
+        eapply wp_ret; [exact Hpc | simregs | ]
+
+    | _ @ _ is ?i  => idtac "Fail with " i; fail
+    end.
+
+  Ltac step :=
+    lazymatch goal with
+    | |- wp _ _ ?f ?pc _ ?n _ =>
+        let H := fresh "Hpc" in
+        eassert (H: f@pc is _) by reflexivity;
+        step_acc H;
+        clear H;
+        destruct n as [|n]; [easy| simpl]; unfold_Prop
+    end.
+
+  Lemma test_inv :
+    NodeInv test 3 (fun v m => v = 10%Z)
+      ⦇fun ρ =>
+         ∃ v,
+         ⌜ρ @ one ⇒ 1⌝ ∧
+         ⌜ρ @ ten ⇒ 10⌝ ∧
+         ⌜ρ @ x ⇒ v⌝ ∧
+         ⌜v <= 10⌝%Z
+      ⦈.
+  Proof using Type.
+    unfold NodeInv.
+    apply löb.
+    intros n m IH ρ (v & Hone & Hten & Hres & Hv); unfold_Prop.
+    step.
+    step.
+    destruct (10 - v =? 0)%Z eqn:He.
+    - step. lia.
+    - step.
+      eapply safe_mono; [|apply IH].
+      + lia.
+      + easy.
+      + exists (v + 1)%Z. repeat split.
+        * simregs.
+        * simregs.
+        * simregs.
+        * lia.
+  Qed.
+
+  Lemma test_correct :
+    hoare P (fun args m => True) test (fun v m => v = 10%Z).
+  Proof using Type.
+    apply hoare_from_wp.
+    intros ρ args H n m _.
+    step.
+    step.
+    step.
+    apply test_inv.
+    - easy.
+    - unfold_Prop.
+      exists 0%Z. repeat split.
+      + simregs.
+      + simregs.
+      + simregs.
+      + lia.
+  Qed.
+
+End Play.
