theories/RTL/SimRules.v
@@ -3,7 +3,6 @@ From RSL Require Import RelLogic Prelude.
 From Coinduction Require Import all.
 
 From RSL Require Import Simulations.FreeSim.
-From RSL Require Import Simulations.FreeSimRules.
 
 From RSL Require Import RTL.RTL.
 From RSL Require Import RTL.Semantics.
@@ -11,7 +10,7 @@ From RSL Require Import RTL.Notations.
 
 Import RTLNotations.
 
-Section Rules.
+Section RulesDef.
   Let Λₜ : lang := rtl_lang.
   Let Λₛ : lang := rtl_lang.
   Context (Pₜ: prog Λₜ) (Pₛ: prog Λₛ).
@@ -33,8 +32,8 @@ Section Rules.
   Definition hoare C ρ P fₜ pcₜ j i fₛ pcₛ Q : Prop :=
     let '(ρₜ, ρₛ) := ρ in
     emp ⊩ ∀ Φ, P -∗
-               (∀ vₜ vₛ, Q vₜ vₛ -∗ Φ vₜ vₛ) -∗
-               sim C ρ fₜ pcₜ j i fₛ pcₛ Φ.
+             (∀ vₜ vₛ, Q vₜ vₛ -∗ Φ vₜ vₛ) -∗
+             sim C ρ fₜ pcₜ j i fₛ pcₛ Φ.
 
   Notation
     "'[' C ']' ρ '⊢' ft '@' pct  '<{' j ',' i '}=' fs '@' pcs '{{' Q '}}'" :=
@@ -57,8 +56,6 @@ Section Rules.
     intros rt vt rs vs Hpct Hpcs Ht Hs.
     intros mtQ msQ HQ.
 
-    unfold regbank_assert, regbank_assert_single in *.
-
     eapply FSourceSteps with (i' := 0).
     { eapply exec_Iret; eassumption. }
 
@@ -70,233 +67,7 @@ Section Rules.
     eapply FRelated.
 
     do 2 eexists; repeat split. simpl.
-    assumption.
-  Qed.
-
-  Lemma source_nop C ρₜ ρₛ P fₜ pcₜ j i fₛ pcₛ Q :
-    ∀ pc,
-    fₛ@pcₛ is <<{ nop -> pc }>> ->
-    [C] (ρₜ, ρₛ) ⊢ {{ P }} fₜ @ pcₜ <{j, 1+i}= fₛ @ pc {{ Q }} ->
-    [C] (ρₜ, ρₛ) ⊢ {{ P }} fₜ @ pcₜ <{j, i}= fₛ @ pcₛ {{ Q }}.
-  Proof using Type.
-    intros pc Hpc H.
-    intros ? ? Hemp Ψ mtPre msPre ? ? Hpre mtPost msPost ? ? Hpost.
-
-    eapply FSourceSteps.
-    - econstructor; eassumption.
-    - now apply H.
-  Qed.
-
-  Lemma target_nop C ρₜ ρₛ P fₜ pcₜ j i fₛ pcₛ Q :
-    ∀ pc,
-    fₜ@pcₜ is <<{ nop -> pc }>> ->
-    [C] (ρₜ, ρₛ) ⊢ {{ P }} fₜ @ pc <{1+j, i}= fₛ @ pcₛ {{ Q }} ->
-    [C] (ρₜ, ρₛ) ⊢ {{ P }} fₜ @ pcₜ <{j, i}= fₛ @ pcₛ {{ Q }}.
-  Proof using Type.
-    intros pc Hpc H.
-    intros ? ? Hemp Ψ mtPre msPre ? ? Hpre mtPost msPost ? ? Hpost.
-
-    eapply FTargetSteps.
-    - eexists. econstructor; eassumption.
-    - intros t Hstep. inv Hstep.
-      eexists. now apply H.
-  Qed.
-
-  Lemma source_op C ρₜ ρₛ P fₜ pcₜ j i fₛ pcₛ Q :
-    ∀ pc dst op regs args v,
-    fₛ@pcₛ is <<{ dst := @op regs -> pc }>> ->
-    ρₛ @ regs ⇒ args ->
-    eval_op op args = Some v ->
-    [C] (ρₜ, ⟦dst ⇐ v⟧ρₛ) ⊢ {{ P }} fₜ @ pcₜ <{j, 1+i}= fₛ @ pc {{ Q }} ->
-    [C] (ρₜ, ρₛ) ⊢ {{ P }} fₜ @ pcₜ <{j, i}= fₛ @ pcₛ {{ Q }}.
-  Proof using Type.
-    intros pc dst op regs args v Hpc Hargs Hv H.
-    intros ? ? Hemp Ψ mtPre msPre ? ? Hpre mtPost msPost ? ? Hpost.
-
-    eapply FSourceSteps.
-    - econstructor; eassumption || reflexivity.
-    - now eapply H.
-  Qed.
-
-  Lemma target_op C ρₜ ρₛ P fₜ pcₜ j i fₛ pcₛ Q :
-    ∀ pc dst op regs args v,
-    fₜ@pcₜ is <<{ dst := @op regs -> pc }>> ->
-    ρₜ @ regs ⇒ args ->
-    eval_op op args = Some v ->
-    [C] (⟦dst ⇐ v⟧ρₜ, ρₛ) ⊢ {{ P }} fₜ @ pc <{1+j, i}= fₛ @ pcₛ {{ Q }} ->
-    [C] (ρₜ, ρₛ) ⊢ {{ P }} fₜ @ pcₜ <{j, i}= fₛ @ pcₛ {{ Q }}.
-  Proof using Type.
-    intros pc dst op regs args v Hpc Hargs Hv H.
-    intros ? ? Hemp Ψ mtPre msPre ? ? Hpre mtPost msPost ? ? Hpost.
-
-    unfold regbank_assert, regbank_assert_list in *.
-
-    eapply FTargetSteps.
-    - eexists. econstructor; eassumption || reflexivity.
-    - intros t Hstep. inv Hstep.
-      eexists. now apply H.
-  Qed.
-
-  Lemma source_load C ρₜ ρₛ P fₜ pcₜ j i fₛ pcₛ Q :
-    ∀ pc dst src addr v,
-    fₛ@pcₛ is <<{ dst := !src -> pc }>> ->
-    ρₛ @ src ⇒ addr ->
-    [C] (ρₜ, ⟦dst ⇐ v⟧ρₛ) ⊢ {{ addr →ₛ v ∗ P }} fₜ @ pcₜ <{j, 1+i}= fₛ @ pc {{ Q }} ->
-    [C] (ρₜ, ρₛ) ⊢ {{ addr →ₛ v ∗ P }} fₜ @ pcₜ <{j, i}= fₛ @ pcₛ {{ Q }}.
-  Proof using Type.
-    intros pc dst src addr v Hpc Haddr H.
-    intros ? ? Hemp Ψ mtPre msPre ? ? Hpre mtPost msPost ? ? Hpost.
-
-    destruct Hpre as (mtAddr & msAddr & mtP & msP & ? & ? & ? & ? & Hm & HP).
-    destruct Hm as (loc & Hloc & Hm).
-
-    eapply FSourceSteps.
-    - eapply exec_Iload with (v := v); try eassumption.
-      + subst. decompose_map_disjoint.
-        unfold get_at. rewrite Hloc.
-        rewrite lookup_union_r, !lookup_union_l by easy.
-        apply lookup_singleton_eq.
-      + reflexivity.
-    - apply H; auto.
-      unfold rlogic_sep.
-      eexists mtAddr, msAddr, mtP, msP.
-      repeat split; auto.
-      eexists. split; eassumption.
-  Qed.
-
-  Lemma target_load C ρₜ ρₛ P fₜ pcₜ j i fₛ pcₛ Q :
-    ∀ pc dst src addr v,
-    fₜ@pcₜ is <<{ dst := !src -> pc }>> ->
-    ρₜ @ src ⇒ addr ->
-    [C] (⟦dst ⇐ v⟧ρₜ, ρₛ) ⊢ {{ addr →ₜ v ∗ P }} fₜ @ pc <{1+j, i}= fₛ @ pcₛ {{ Q }} ->
-    [C] (ρₜ, ρₛ) ⊢ {{ addr →ₜ v ∗ P }} fₜ @ pcₜ <{j, i}= fₛ @ pcₛ {{ Q }}.
-  Proof using Type.
-    intros pc dst src addr v Hpc Haddr H.
-    intros ? ? Hemp Ψ mtPre msPre ? ? Hpre mtPost msPost ? ? Hpost.
-
-    unfold regbank_assert, regbank_assert_single in Haddr.
-    destruct Hpre as (mtAddr & msAddr & mtP & msP & ? & ? & ? & ? & Hm & HP).
-    destruct Hm as (loc & Hloc & Hm).
-
-    eapply FTargetSteps.
-    - eexists. eapply exec_Iload; try eassumption.
-      + subst. decompose_map_disjoint.
-        unfold get_at. rewrite Hloc.
-        rewrite lookup_union_r, !lookup_union_l, lookup_singleton_eq by easy.
-        reflexivity.
-      + reflexivity.
-    - subst. decompose_map_disjoint.
-      intros t Hstep.
-      inv Hstep as [ | | | ? ? ? ? ? ? ? ? ? ? ? ? ? Hget | | | | | ].
-
-      unfold get_at in Hget. rewrite Hloc in Hget.
-      rewrite lookup_union_r, !lookup_union_l, lookup_singleton_eq
-                in Hget by easy.
-      injection Hget as <-.
-
-      eexists. apply H; try solve_map_disjoint.
-      eexists _, msAddr, mtP, msP. repeat split; eauto.
-      + solve_map_disjoint.
-      + exists loc. now split.
-  Qed.
-
-  Lemma source_store C ρₜ ρₛ P fₜ pcₜ j i fₛ pcₛ Q :
-    ∀ pc dst src addr v old,
-    fₛ@pcₛ is <<{ !dst := src -> pc }>> ->
-    ρₛ @ dst ⇒ addr ->
-    ρₛ @ src ⇒ v ->
-    [C] (ρₜ, ρₛ) ⊢ {{ addr →ₛ v ∗ P }} fₜ @ pcₜ <{j, 1+i}= fₛ @ pc {{ Q }} ->
-    [C] (ρₜ, ρₛ) ⊢ {{ addr →ₛ old ∗ P }} fₜ @ pcₜ <{j, i}= fₛ @ pcₛ {{ Q }}.
-  Proof using Type.
-    intros pc dst src addr v old Hpc Haddr Hv H.
-    intros ? ? Hemp Ψ mtPre msPre ? ? Hpre mtPost msPost ? ? Hpost.
-
-    unfold regbank_assert, regbank_assert_single in Haddr, Hv.
-    destruct Hpre as (mtAddr & msAddr & mtP & msP & ? & ? & ? & ? & Hm & HP).
-    destruct Hm as (loc & Hloc & Hm).
-
-    eapply FSourceSteps.
-    - eapply exec_Istore; try eassumption.
-      subst. decompose_map_disjoint.
-      unfold set_at, update_at. rewrite Hloc.
-      rewrite alter_union_right, !alter_union_left, alter_singleton_eq;
-      solve_map_disjoint.
-
-    - subst. decompose_map_disjoint.
-      eapply H; try solve_map_disjoint.
-      eexists mtAddr, _, mtP, msP. repeat split; eauto.
-      + solve_map_disjoint.
-      + exists loc. now split.
-  Qed.
-
-  Lemma target_store C ρₜ ρₛ P fₜ pcₜ j i fₛ pcₛ Q :
-    ∀ pc dst src addr v old,
-    fₜ@pcₜ is <<{ !dst := src -> pc }>> ->
-    ρₜ @ dst ⇒ addr ->
-    ρₜ @ src ⇒ v ->
-    [C] (ρₜ, ρₛ) ⊢ {{ addr →ₜ v ∗ P }} fₜ @ pc <{1+j, i}= fₛ @ pcₛ {{ Q }} ->
-    [C] (ρₜ, ρₛ) ⊢ {{ addr →ₜ old ∗ P }} fₜ @ pcₜ <{j, i}= fₛ @ pcₛ {{ Q }}.
-  Proof using Type.
-    intros pc dst src addr v old Hpc Haddr Hv H.
-    intros ? ? Hemp Ψ mtPre msPre ? ? Hpre mtPost msPost ? ? Hpost.
-
-    unfold regbank_assert, regbank_assert_single in Haddr, Hv.
-    destruct Hpre as (mtAddr & msAddr & mtP & msP & ? & ? & ? & ? & Hm & HP).
-    destruct Hm as (loc & Hloc & Hm).
-
-    eapply FTargetSteps.
-    - eexists. eapply exec_Istore; try eassumption.
-      unfold set_at, update_at. now rewrite Hloc.
-    - intros t Hstep.
-      inv Hstep as [ | | | | ? ? ? ? ? ? ? ? ? ? ? ? ? ? Hset | | | | ].
-
-      unfold set_at, update_at in Hset. rewrite Hloc in Hset.
-      rewrite alter_union_right, !alter_union_left, alter_singleton_eq
-                in Hset by solve_map_disjoint.
-      injection Hset as Hset.
-
-      subst. decompose_map_disjoint.
-      eexists. apply H; try solve_map_disjoint.
-      + eexists _, msAddr, mtP, msP. repeat split; eauto.
-        * solve_map_disjoint.
-        * exists loc. now split.
-  Qed.
-
-  Lemma source_if C ρₜ ρₛ P fₜ pcₜ j i fₛ pcₛ Q :
-    ∀ pc_true pc_false reg v pc,
-    fₛ@pcₛ is <<{ if reg then goto pc_true else goto pc_false }>> ->
-    ρₛ @ reg ⇒ v ->
-    (if (v =? 0)%Z then pc_true else pc_false) = pc ->
-    [C] (ρₜ, ρₛ) ⊢ {{ P }} fₜ @ pcₜ <{j, 1+i}= fₛ @ pc {{ Q }} ->
-    [C] (ρₜ, ρₛ) ⊢ {{ P }} fₜ @ pcₜ <{j, i}= fₛ @ pcₛ {{ Q }}.
-  Proof using Type.
-    intros pc_true pc_false reg v pc Hpc Hv Hnext_pc H.
-    intros ? ? Hemp Ψ mtPre msPre ? ? Hpre mtPost msPost ? ? Hpost.
-
-    unfold regbank_assert, regbank_assert_single in Hv.
-
-    eapply FSourceSteps.
-    - econstructor; eassumption || reflexivity.
-    - subst. now apply H.
-  Qed.
-
-  Lemma target_if C ρₜ ρₛ P fₜ pcₜ j i fₛ pcₛ Q :
-    ∀ pc_true pc_false reg v pc,
-    fₜ@pcₜ is <<{ if reg then goto pc_true else goto pc_false }>> ->
-    ρₜ @ reg ⇒ v ->
-    (if (v =? 0)%Z then pc_true else pc_false) = pc ->
-    [C] (ρₜ, ρₛ) ⊢ {{ P }} fₜ @ pc <{1+j, i}= fₛ @ pcₛ {{ Q }} ->
-    [C] (ρₜ, ρₛ) ⊢ {{ P }} fₜ @ pcₜ <{j, i}= fₛ @ pcₛ {{ Q }}.
-  Proof using Type.
-    intros pc_true pc_false reg v pc Hpc Hv Hnext_pc H.
-    intros ? ? Hemp Ψ mtPre msPre ? ? Hpre mtPost msPost ? ? Hpost.
-
-    unfold regbank_assert, regbank_assert_single in Hv.
-
-    eapply FTargetSteps.
-    - eexists. econstructor; eassumption || reflexivity.
-    - intros t Hstep. inv Hstep.
-      eexists. now apply H.
+    simregs. assumption.
   Qed.
 
   Lemma frame C ρₜ ρₛ P1 P2 fₜ pcₜ j i fₛ pcₛ Q :
@@ -375,6 +146,7 @@ Section Rules.
     - intros ? ? Hemp Ψ mtPre msPre ? ? Hpre mtPost msPost ? ? Hpost.
       destruct Hemp as (-> & ->).
       decompose_map_disjoint.
+      unfold memory in *.
       rewrite !(map_union_empty _).
       apply H with (Ψ := fun '(vₜ, mₜ) '(vₛ, mₛ) => Ψ vₜ vₛ mₜ mₛ).
       repeat split; easy.
@@ -425,7 +197,7 @@ Section Rules.
     - assumption.
     - solve_map_disjoint.
     - solve_map_disjoint.
-    - assumption.
+    - intros vₜ vₛ mt ms. apply Hpost.
   Qed.
 
   Lemma iex C ρₜ ρₛ fₜ pcₜ j i fₛ pcₛ Q :
@@ -460,7 +232,7 @@ Section Rules.
       + assumption.
       + solve_map_disjoint.
       + solve_map_disjoint.
-      + now rewrite !(map_empty_union _).
+      + unfold memory in *. now rewrite !(map_empty_union _).
     - intros H HP1.
       intros ? ? Hemp Ψ mtPre msPre ? ? Hpre.
       eapply H.
@@ -474,18 +246,22 @@ Section Rules.
         * apply map_empty_union.
   Qed.
 
-  Lemma index_mono (C: Chain fsim_lfp) ρₜ ρₛ P fₜ pcₜ j i fₛ pcₛ Q :
+  Lemma fsim_mono ρₜ ρₛ P fₜ pcₜ j i fₛ pcₛ Q :
     ∀ j' i',
     (j' <= j)%nat ->
     (i' <= i)%nat ->
-    [elem C] (ρₜ, ρₛ) ⊢ {{ P }} fₜ @ pcₜ <{j', i'}= fₛ @ pcₛ {{ Q }} ->
-    [elem C] (ρₜ, ρₛ) ⊢ {{ P }} fₜ @ pcₜ <{j, i}= fₛ @ pcₛ {{ Q }}.
+    [fsim] (ρₜ, ρₛ) ⊢ {{ P }} fₜ @ pcₜ <{j', i'}= fₛ @ pcₛ {{ Q }} ->
+    [fsim] (ρₜ, ρₛ) ⊢ {{ P }} fₜ @ pcₜ <{j, i}= fₛ @ pcₛ {{ Q }}.
   Proof using Type.
     intros i' j' Hi Hj H.
     intros ? ? Hemp Ψ mtPre msPre ? ? Hpre mtPost msPost ? ? Hpost.
+    apply (gfp_fp fsim_lfp).
     eapply idx_mono.
-    - now apply H.
+    - apply (gfp_chain (chain_gfp fsim_lfp)).
+      apply (gfp_fp fsim_lfp).
+      now apply H.
     - unfold "⊑". simpl. lia.
     - unfold "⊑". simpl. lia.
   Qed.
-End Rules.
+
+End RulesDef.
