theories/RTL/SourceRules.v
@@ -1,0 +1,137 @@
+From RSL Require Import RelLogic Prelude.
+
+From Coinduction Require Import all.
+
+From RSL Require Import Simulations.FreeSim.
+From RSL Require Import Simulations.FreeSimRules.
+
+From RSL Require Import RTL.RTL.
+From RSL Require Import RTL.Semantics.
+From RSL Require Import RTL.Notations.
+From RSL Require Import RTL.SimRules.
+
+From RSL Require Import Tactics.Memory.
+
+Import RTLNotations.
+
+Section SourceRulesDef.
+  Let Λₜ : lang := rtl_lang.
+  Let Λₛ : lang := rtl_lang.
+  Context (Pₜ: prog Λₜ) (Pₛ: prog Λₛ).
+
+  Abbreviation fsim := (fsim WfNat WfNat Pₜ Pₛ).
+
+  Notation
+    "'[' C ']' ρ '⊢' ft '@' pct  '<{' j ',' i '}=' fs '@' pcs '{{' Q '}}'" :=
+    (sim Pₜ Pₛ C ρ ft pct j i fs pcs Q%rlogic)
+      (at level 0, ft at level 0, fs at level 0, no associativity).
+
+  Notation
+    "'[' C ']' ρ '⊢' '{{' P '}}' ft '@' pct  '<{' j ',' i '}=' fs '@' pcs '{{' Q '}}'" :=
+    (hoare Pₜ Pₛ C ρ P%rlogic ft pct j i fs pcs Q%rlogic)
+      (at level 0, ft at level 0, fs at level 0, no associativity).
+
+  Lemma source_nop C ρₜ ρₛ P fₜ pcₜ j i fₛ pcₛ Q :
+    ∀ pc,
+    fₛ@pcₛ is <<{ nop -> pc }>> ->
+    [C] (ρₜ, ρₛ) ⊢ {{ P }} fₜ @ pcₜ <{j, 1+i}= fₛ @ pc {{ Q }} ->
+    [C] (ρₜ, ρₛ) ⊢ {{ P }} fₜ @ pcₜ <{j, i}= fₛ @ pcₛ {{ Q }}.
+  Proof using Type.
+    intros pc Hpc H.
+    intros ? ? Hemp Ψ mtPre msPre ? ? Hpre mtPost msPost ? ? Hpost.
+
+    eapply FSourceSteps.
+    - econstructor; eassumption.
+    - now apply H.
+  Qed.
+
+  Lemma source_op C ρₜ ρₛ P fₜ pcₜ j i fₛ pcₛ Q :
+    ∀ pc dst op regs args,
+    fₛ@pcₛ is <<{ dst := @op regs -> pc }>> ->
+    ρₛ @ regs ⇒ args ->
+    (∀ v, eval_op op args = Some v ->
+     [C] (ρₜ, ⟦dst ⇐ v⟧ρₛ) ⊢ {{ P }} fₜ @ pcₜ <{j, 1+i}= fₛ @ pc {{ Q }}) ->
+    [C] (ρₜ, ρₛ) ⊢ {{ P }} fₜ @ pcₜ <{j, i}= fₛ @ pcₛ {{ Q }}.
+  Proof using Type.
+    intros pc dst op regs args Hpc Hargs H.
+    intros ? ? Hemp Ψ mtPre msPre ? ? Hpre mtPost msPost ? ? Hpost.
+
+    destruct (eval_op op args) as [v|] eqn:Hv.
+    - eapply FSourceSteps.
+      + econstructor; eassumption || reflexivity.
+      + now eapply H.
+    - apply FSourceStuck.
+      split.
+      { reflexivity. }
+      intros Hprog. apply can_progress_must_step in Hprog.
+      destruct Hprog as [? Hprog].
+      inv Hprog. simregs.
+  Qed.
+
+  Lemma source_load C ρₜ ρₛ P fₜ pcₜ j i fₛ pcₛ Q :
+    ∀ pc dst src addr v,
+    fₛ@pcₛ is <<{ dst := !src -> pc }>> ->
+    ρₛ @ src ⇒ addr ->
+    [C] (ρₜ, ⟦dst ⇐ v⟧ρₛ) ⊢ {{ addr →ₛ v ∗ P }} fₜ @ pcₜ <{j, 1+i}= fₛ @ pc {{ Q }} ->
+    [C] (ρₜ, ρₛ) ⊢ {{ addr →ₛ v ∗ P }} fₜ @ pcₜ <{j, i}= fₛ @ pcₛ {{ Q }}.
+  Proof using Type.
+    intros pc dst src addr v Hpc Haddr H.
+    intros ? ? Hemp Ψ mtPre msPre ? ? Hpre mtPost msPost ? ? Hpost.
+
+    destruct Hpre as (mtAddr & msAddr & mtP & msP & ? & ? & ? & ? & Hm & HP).
+    destruct Hm as (Ht & (l & Hl & Hs)).
+
+    eapply FSourceSteps.
+    - eapply exec_Iload with (v := v); try eassumption.
+      + subst. now simget.
+      + reflexivity.
+    - apply H; auto.
+      eexists mtAddr, msAddr, mtP, msP.
+      repeat split; auto.
+      eexists. split; eassumption.
+  Qed.
+
+  Lemma source_store C ρₜ ρₛ P fₜ pcₜ j i fₛ pcₛ Q :
+    ∀ pc dst src addr v old,
+    fₛ@pcₛ is <<{ !dst := src -> pc }>> ->
+    ρₛ @ dst ⇒ addr ->
+    ρₛ @ src ⇒ v ->
+    [C] (ρₜ, ρₛ) ⊢ {{ addr →ₛ v ∗ P }} fₜ @ pcₜ <{j, 1+i}= fₛ @ pc {{ Q }} ->
+    [C] (ρₜ, ρₛ) ⊢ {{ addr →ₛ old ∗ P }} fₜ @ pcₜ <{j, i}= fₛ @ pcₛ {{ Q }}.
+  Proof using Type.
+    intros pc dst src addr v old Hpc Haddr Hv H.
+    intros ? ? Hemp Ψ mtPre msPre ? ? Hpre mtPost msPost ? ? Hpost.
+
+    destruct Hpre as (mtAddr & msAddr & mtP & msP & ? & ? & ? & ? & Hm & HP).
+    destruct Hm as (Ht & (l & Hl & Hs)).
+
+    eapply FSourceSteps.
+    - eapply exec_Istore; try eassumption.
+      subst. erewrite (set_at_some  _ _ _ _ _ Hl) by now simget.
+      rewrite !alter_union_right by solve_map_disjoint.
+      rewrite !alter_union_left by solve_map_disjoint.
+      rewrite !alter_singleton.
+      reflexivity.
+    - subst. apply H; try solve_map_disjoint.
+      eexists ∅, _, mtP, msP. repeat split; eauto.
+      + solve_map_disjoint.
+      + exists l. now split.
+  Qed.
+
+  Lemma source_if C ρₜ ρₛ P fₜ pcₜ j i fₛ pcₛ Q :
+    ∀ pc_true pc_false reg v pc,
+    fₛ@pcₛ is <<{ if reg then goto pc_true else goto pc_false }>> ->
+    ρₛ @ reg ⇒ v ->
+    (if (v =? 0)%Z then pc_true else pc_false) = pc ->
+    [C] (ρₜ, ρₛ) ⊢ {{ P }} fₜ @ pcₜ <{j, 1+i}= fₛ @ pc {{ Q }} ->
+    [C] (ρₜ, ρₛ) ⊢ {{ P }} fₜ @ pcₜ <{j, i}= fₛ @ pcₛ {{ Q }}.
+  Proof using Type.
+    intros pc_true pc_false reg v pc Hpc Hv Hnext_pc H.
+    intros ? ? Hemp Ψ mtPre msPre ? ? Hpre mtPost msPost ? ? Hpost.
+
+    eapply FSourceSteps.
+    - econstructor; eassumption || reflexivity.
+    - subst. now apply H.
+  Qed.
+
+End SourceRulesDef.
