theories/RTL/TargetRules.v
@@ -1,0 +1,145 @@
+From RSL Require Import RelLogic Prelude.
+
+From Coinduction Require Import all.
+
+From RSL Require Import Simulations.FreeSim.
+From RSL Require Import Simulations.FreeSimRules.
+
+From RSL Require Import RTL.RTL.
+From RSL Require Import RTL.Semantics.
+From RSL Require Import RTL.Notations.
+From RSL Require Import RTL.SimRules.
+
+From RSL Require Import Tactics.Memory.
+
+Import RTLNotations.
+
+Section TargetRulesDef.
+  Let Λₜ : lang := rtl_lang.
+  Let Λₛ : lang := rtl_lang.
+  Context (Pₜ: prog Λₜ) (Pₛ: prog Λₛ).
+
+  Abbreviation fsim := (fsim WfNat WfNat Pₜ Pₛ).
+
+  Notation
+    "'[' C ']' ρ '⊢' ft '@' pct  '<{' j ',' i '}=' fs '@' pcs '{{' Q '}}'" :=
+    (sim Pₜ Pₛ C ρ ft pct j i fs pcs Q%rlogic)
+      (at level 0, ft at level 0, fs at level 0, no associativity).
+
+  Notation
+    "'[' C ']' ρ '⊢' '{{' P '}}' ft '@' pct  '<{' j ',' i '}=' fs '@' pcs '{{' Q '}}'" :=
+    (hoare Pₜ Pₛ C ρ P%rlogic ft pct j i fs pcs Q%rlogic)
+      (at level 0, ft at level 0, fs at level 0, no associativity).
+
+  Lemma target_nop C ρₜ ρₛ P fₜ pcₜ j i fₛ pcₛ Q :
+    ∀ pc,
+    fₜ@pcₜ is <<{ nop -> pc }>> ->
+    [C] (ρₜ, ρₛ) ⊢ {{ P }} fₜ @ pc <{1+j, i}= fₛ @ pcₛ {{ Q }} ->
+    [C] (ρₜ, ρₛ) ⊢ {{ P }} fₜ @ pcₜ <{j, i}= fₛ @ pcₛ {{ Q }}.
+  Proof using Type.
+    intros pc Hpc H.
+    intros ? ? Hemp Ψ mtPre msPre ? ? Hpre mtPost msPost ? ? Hpost.
+
+    eapply FTargetSteps.
+    - eexists. econstructor; eassumption.
+    - intros t Hstep. inv Hstep.
+      eexists. now apply H.
+  Qed.
+
+  Lemma target_op C ρₜ ρₛ P fₜ pcₜ j i fₛ pcₛ Q :
+    ∀ pc dst op regs args v,
+    fₜ@pcₜ is <<{ dst := @op regs -> pc }>> ->
+    ρₜ @ regs ⇒ args ->
+    eval_op op args = Some v ->
+    [C] (⟦dst ⇐ v⟧ρₜ, ρₛ) ⊢ {{ P }} fₜ @ pc <{1+j, i}= fₛ @ pcₛ {{ Q }} ->
+    [C] (ρₜ, ρₛ) ⊢ {{ P }} fₜ @ pcₜ <{j, i}= fₛ @ pcₛ {{ Q }}.
+  Proof using Type.
+    intros pc dst op regs args v Hpc Hargs Hv H.
+    intros ? ? Hemp Ψ mtPre msPre ? ? Hpre mtPost msPost ? ? Hpost.
+
+    eapply FTargetSteps.
+    - eexists. econstructor; eassumption || reflexivity.
+    - intros t Hstep. inv Hstep. simregs.
+      eexists. now apply H.
+  Qed.
+
+  Lemma target_load C ρₜ ρₛ P fₜ pcₜ j i fₛ pcₛ Q :
+    ∀ pc dst src addr v,
+    fₜ@pcₜ is <<{ dst := !src -> pc }>> ->
+    ρₜ @ src ⇒ addr ->
+    [C] (⟦dst ⇐ v⟧ρₜ, ρₛ) ⊢ {{ addr →ₜ v ∗ P }} fₜ @ pc <{1+j, i}= fₛ @ pcₛ {{ Q }} ->
+    [C] (ρₜ, ρₛ) ⊢ {{ addr →ₜ v ∗ P }} fₜ @ pcₜ <{j, i}= fₛ @ pcₛ {{ Q }}.
+  Proof using Type.
+    intros pc dst src addr v Hpc Haddr H.
+    intros ? ? Hemp Ψ mtPre msPre ? ? Hpre mtPost msPost ? ? Hpost.
+
+    destruct Hpre as (mtAddr & msAddr & mtP & msP & ? & ? & ? & ? & Hm & HP).
+    destruct Hm as ((l & Hl & Ht) & Hs).
+
+    eapply FTargetSteps.
+    - eexists. eapply exec_Iload; try eassumption.
+      + subst. now simget.
+      + reflexivity.
+    - subst.
+      intros t Hstep.
+      inv Hstep. simregs. simget. subst.
+
+      eexists. apply H; try solve_map_disjoint.
+      eexists _, ∅, mtP, msP. repeat split; eauto.
+      exists l. now split.
+  Qed.
+
+  Lemma target_store C ρₜ ρₛ P fₜ pcₜ j i fₛ pcₛ Q :
+    ∀ pc dst src addr v old,
+    fₜ@pcₜ is <<{ !dst := src -> pc }>> ->
+    ρₜ @ dst ⇒ addr ->
+    ρₜ @ src ⇒ v ->
+    [C] (ρₜ, ρₛ) ⊢ {{ addr →ₜ v ∗ P }} fₜ @ pc <{1+j, i}= fₛ @ pcₛ {{ Q }} ->
+    [C] (ρₜ, ρₛ) ⊢ {{ addr →ₜ old ∗ P }} fₜ @ pcₜ <{j, i}= fₛ @ pcₛ {{ Q }}.
+  Proof using Type.
+    intros pc dst src addr v old Hpc Haddr Hv H.
+    intros ? ? Hemp Ψ mtPre msPre ? ? Hpre mtPost msPost ? ? Hpost.
+
+    destruct Hpre as (mtAddr & msAddr & mtP & msP & ? & ? & ? & ? & Hm & HP).
+    destruct Hm as ((l & Hl & Ht) & Hs).
+
+    eapply FTargetSteps.
+    - eexists. eapply exec_Istore; try eassumption.
+      subst.
+      erewrite (set_at_some  _ _ _ _ _ Hl) by simget.
+      rewrite !alter_union_right, !alter_union_left, alter_singleton by solve_map_disjoint.
+      reflexivity.
+    - intros t Hstep.
+      inv Hstep.
+      simregs.
+      erewrite (set_at_some  _ _ _ _ _ Hl) in * by simget.
+      rewrite !alter_union_right, !alter_union_left, alter_singleton
+                in * by solve_map_disjoint.
+      rewrite inj_some in *.
+
+      subst. decompose_map_disjoint.
+      eexists. apply H; try solve_map_disjoint.
+      eexists _, ∅, mtP, msP. repeat split; eauto.
+      + solve_map_disjoint.
+      + solve_map_disjoint.
+      + exists l. now split.
+  Qed.
+
+  Lemma target_if C ρₜ ρₛ P fₜ pcₜ j i fₛ pcₛ Q :
+    ∀ pc_true pc_false reg v pc,
+    fₜ@pcₜ is <<{ if reg then goto pc_true else goto pc_false }>> ->
+    ρₜ @ reg ⇒ v ->
+    (if (v =? 0)%Z then pc_true else pc_false) = pc ->
+    [C] (ρₜ, ρₛ) ⊢ {{ P }} fₜ @ pc <{1+j, i}= fₛ @ pcₛ {{ Q }} ->
+    [C] (ρₜ, ρₛ) ⊢ {{ P }} fₜ @ pcₜ <{j, i}= fₛ @ pcₛ {{ Q }}.
+  Proof using Type.
+    intros pc_true pc_false reg v pc Hpc Hv Hnext_pc H.
+    intros ? ? Hemp Ψ mtPre msPre ? ? Hpre mtPost msPost ? ? Hpost.
+
+    eapply FTargetSteps.
+    - eexists. econstructor; eassumption || reflexivity.
+    - intros t Hstep. inv Hstep. simregs.
+      eexists. now apply H.
+  Qed.
+
+End TargetRulesDef.
