theories/RelLogic/Memory.v
@@ -3,46 +3,35 @@ From RSL Require Import RelLogic.Logic.
 
 (** ** Memory Connectives *)
 
-Section MemoryOp.
-  Definition rlogic_mem_t_assert addr v : rlogic :=
-    fun mt _ =>
-      ∃ loc, val_to_loc addr = Some loc ∧ mt = {[loc := v]}.
+Local Definition mem_assert addr x (m: memory) : Prop :=
+  ∃ loc, val_to_loc addr = Some loc ∧ m = {[loc := x]}.
 
-  Definition rlogic_mem_s_assert addr v : rlogic :=
-    fun _ ms =>
-      ∃ loc, val_to_loc addr = Some loc ∧ ms = {[loc := v]}.
+Definition rlogic_mem_t_assert addr x : rlogic :=
+  fun mt ms => mem_assert addr x mt ∧ ms = ∅.
 
-  Definition rlogic_mem_same_at P addrt addrs : rlogic :=
-    fun mt ms =>
-      ∃ loct locs vt vs,
-        val_to_loc addrt = Some loct ∧
-        val_to_loc addrs = Some locs ∧
-        mt = {[loct := vt]} ∧
-        ms = {[locs := vs]} ∧
-        P vt vs.
-
-End MemoryOp.
+Definition rlogic_mem_s_assert addr x : rlogic :=
+  fun mt ms => mt = ∅ ∧ mem_assert addr x ms.
 
 Notation "l '→ₜ' v" :=
-  (rlogic_mem_t_assert l%positive v%Z)
+  ⦇ rlogic_mem_t_assert l%positive v%Z ⦈
     (at level 70, no associativity, format "l →ₜ v") : rlogic_scope.
 
 Notation "l '→ₛ' v" :=
-  (rlogic_mem_s_assert l%positive v%Z)
+  ⦇ rlogic_mem_s_assert l%positive v%Z ⦈
     (at level 70, no associativity, format "l →ₛ v") : rlogic_scope.
 
 Notation "addrt 'ₜ⟨' P '⟩ₛ' addrs" :=
-  (rlogic_mem_same_at P addrt%positive addrs%positive)
+  ⦇ ∃ vt vs, addrt →ₜ vt ∗ addrs →ₛ vs ∗ ⌜P vt vs⌝ ⦈
     (at level 70, no associativity) : rlogic_scope.
 
 Notation "addrs 'ₛ⟨' P '⟩ₜ' addrt" :=
-  (rlogic_mem_same_at P addrt%positive addrs%positive)
+  ⦇ ∃ vt vs, addrt →ₜ vt ∗ addrs →ₛ vs ∗ ⌜P vt vs⌝ ⦈
     (at level 70, no associativity) : rlogic_scope.
 
 Notation "addrt 'ₜ~ₛ' addrs" :=
-  (rlogic_mem_same_at eq addrt%positive addrs%positive)
+  ⦇ ∃ v, addrt →ₜ v ∗ addrs →ₛ v ⦈
     (at level 70, no associativity) : rlogic_scope.
 
 Notation "addrs 'ₛ~ₜ' addrt" :=
-  (rlogic_mem_same_at eq addrt%positive addrs%positive)
+  ⦇ ∃ v, addrt →ₜ v ∗ addrs →ₛ v ⦈
     (at level 70, no associativity) : rlogic_scope.
