theories/Tactics/Memory.v
@@ -1,0 +1,232 @@
+From RSL Require Import Prelude.
+
+From stdpp Require Import fin_maps.
+
+From Ltac2 Require Import Ltac2.
+From Ltac2 Require Import Printf.
+From Ltac2 Require Import Notations.
+
+Lemma get_at_union_left addr l (m1 m2: memory) :
+  val_to_loc addr = Some l ->
+  m1 ##ₘ m2 ->
+  m2 !! l = None ->
+  get_at addr (m1 ∪ m2) = get_at addr m1.
+Proof.
+  intros Hloc Hdij Hmem.
+  unfold get_at. rewrite Hloc.
+  unfold memory in *.
+  now rewrite lookup_union_l.
+Qed.
+
+Lemma get_at_union_right addr l (m1 m2: memory) :
+  val_to_loc addr = Some l ->
+  m1 ##ₘ m2 ->
+  m1 !! l = None ->
+  get_at addr (m1 ∪ m2) = get_at addr m2.
+Proof.
+  intros Hloc Hdij Hmem.
+  unfold get_at. rewrite Hloc.
+  unfold memory in *.
+  now rewrite lookup_union_r.
+Qed.
+
+Lemma get_at_singl addr l v :
+  val_to_loc addr = Some l ->
+  get_at addr {[ l := v ]} = Some v.
+Proof.
+  intros Hloc.
+  unfold get_at. rewrite Hloc.
+  unfold memory in *.
+  now rewrite lookup_singleton_eq.
+Qed.
+
+(** A small utility to print the goal *)
+Ltac2 print_goal () :=
+  let g := Control.goal () in
+  Message.print (Message.of_constr g).
+
+Ltac2 rec first_of tacs : unit :=
+  match tacs with
+  | [] => Control.backtrack_tactic_failure "Empty first list"
+  | tac :: tacs =>
+      Control.enter (fun _ => orelse tac (fun _ => first_of tacs))
+  end.
+
+Ltac2 assert_by h cst tac :=
+  Std.assert
+    (Std.AssertType
+       (Some (Std.IntroNaming (Std.IntroIdentifier h)))
+       cst
+       (Some tac)).
+
+(* Ltac2 debug (tac: unit -> unit) () : unit := *)
+(*   match Control.case tac with *)
+(*   | Val (x, k) => Control.plus (fun () => x) k *)
+(*   | Err e => *)
+(*       let einfo := Control.current_exninfo () *)
+(*       in Control.throw_bt (Debug (Control.print_exn e)) einfo *)
+(*   end. *)
+
+Ltac2 in_hyp h : Std.clause :=
+  {
+    Std.on_hyps := Some [(h, Std.AllOccurrences, Std.InHyp)];
+    Std.on_concl := Std.NoOccurrences
+  }.
+
+Ltac2 in_goal : Std.clause :=
+  {
+    Std.on_hyps := Some [];
+    Std.on_concl := Std.AllOccurrences
+  }.
+
+Ltac2 rewrite_in_hyp thm hyps cl tac :=
+  Std.rewrite false
+    [{
+      Std.rew_orient := None;
+      Std.rew_repeat := Std.Precisely 1;
+      Std.rew_equatn :=
+              (fun () => (thm, Std.ExplicitBindings hyps))
+    }]
+    cl
+    tac.
+
+Ltac2 call_solve_disjoint () : unit :=
+  Control.enter (fun () => ltac1:(solve_map_disjoint)).
+
+Ltac2 simgetpair hloc m1 m2 place : unit :=
+  let hdij := Fresh.in_goal @Hdij in
+  assert_by hdij '($m1 ##ₘ $m2) call_solve_disjoint;
+  first_of [
+      (fun () => rewrite_in_hyp 'get_at_union_left
+                 [(Std.AnonHyp 1, Control.hyp hloc);
+                  (Std.AnonHyp 2, Control.hyp hdij)]
+                 place (Some call_solve_disjoint));
+      (fun () => rewrite_in_hyp 'get_at_union_right
+                 [(Std.AnonHyp 1, Control.hyp hloc);
+                  (Std.AnonHyp 2, Control.hyp hdij)]
+                 place (Some call_solve_disjoint))
+    ];
+  Std.clear [hdij].
+
+Ltac2 discr_or_inj h :=
+  first_of [
+      (fun () =>
+         Std.injection
+           false
+           (Some [Std.IntroNaming (Std.IntroIdentifier h)])
+           (Some (Std.ElimOnIdent h))
+      );
+      (fun () =>
+         Std.discriminate false (Some (Std.ElimOnIdent h))
+      );
+      (fun _ => ())
+    ].
+
+Ltac2 rec simget0 () : unit :=
+  lazy_match! goal with
+  | [hloc: val_to_loc ?_addr = Some _,
+       hget: get_at ?_addr ?m = _ |- _] =>
+      lazy_match! m with
+      | ?m1 ∪ ?m2 =>
+          simgetpair hloc m1 m2 (in_hyp hget);
+          try0 simget0
+      | {[_ := _ ]} =>
+          rewrite_in_hyp 'get_at_singl
+            [(Std.AnonHyp 1, Control.hyp hloc)] (in_hyp hget) None;
+          discr_or_inj hget
+      end
+  | [hloc: val_to_loc ?_addr = Some _ |- get_at ?_addr ?m = _ ] =>
+      lazy_match! m with
+      | ?m1 ∪ ?m2 =>
+          simgetpair hloc m1 m2 in_goal;
+          try0 simget0
+      | {[_ := _ ]} =>
+          rewrite_in_hyp 'get_at_singl
+            [(Std.AnonHyp 1, Control.hyp hloc)] in_goal None;
+          try0 Std.reflexivity
+      end
+  end.
+
+Ltac simget :=
+  match goal with
+  | [hloc: val_to_loc ?_addr = Some _,
+       hget: get_at ?_addr ?m = _ |- _] =>
+      rewrite
+        !(get_at_union_right _ _ _ _ hloc),
+        !(get_at_union_left _ _ _ _ hloc),
+        !(get_at_singl _ _ _ hloc)
+          in hget by solve_map_disjoint;
+      inv hget
+  | [hloc: val_to_loc ?_addr = Some _
+     |- get_at ?_addr ?m = _ ] =>
+      rewrite
+        !(get_at_union_right _ _ _ _ hloc),
+        !(get_at_union_left _ _ _ _ hloc),
+        !(get_at_singl _ _ _ hloc)
+            by solve_map_disjoint;
+      try easy
+  end.
+
+Lemma set_at_some addr l v old m:
+  val_to_loc addr = Some l ->
+  get_at addr m = Some old ->
+  set_at addr v m = Some (alter (fun _ => v) l m).
+Proof.
+  unfold set_at, get_at.
+  intros Hloc Hget.
+  rewrite Hloc in *.
+  destruct (m !! l) as [[]|]; congruence.
+Qed.
+
+Lemma set_at_none addr v m:
+  get_at addr m = None ->
+  set_at addr v m = None.
+Proof.
+  unfold set_at, get_at.
+  intros Hget.
+  destruct (val_to_loc addr) as [l|].
+  - destruct (m !! l) as [[]|]; congruence.
+  - reflexivity.
+Qed.
+
+Lemma alter_union_right f l (m1 m2: memory) :
+  m1 ##ₘ m2 ->
+  m1 !! l = None ->
+  alter f l (m1 ∪ m2) = m1 ∪ alter f l m2.
+Proof using Type.
+  intros Hdij Hnin.
+  unfold union, map_union.
+  rewrite (alter_union_with_r _ _ m1).
+  - reflexivity.
+  - intros x y H1 H2. exfalso.
+    rewrite map_disjoint_alt in Hdij.
+    destruct (Hdij l) as [? | ?]; congruence.
+  - intros x H1 H2.
+    unfold memory in *.
+    congruence.
+Qed.
+
+Lemma alter_union_left f l (m1 m2: memory) :
+  m1 ##ₘ m2 ->
+  m2 !! l = None ->
+  alter f l (m1 ∪ m2) = alter f l m1 ∪ m2.
+Proof using Type.
+  intros Hdij Hnin.
+  unfold union, map_union.
+  rewrite (alter_union_with_l _ _ m1).
+  - reflexivity.
+  - intros x y H1 H2. exfalso.
+    rewrite map_disjoint_alt in Hdij.
+    destruct (Hdij l) as [? | ?]; congruence.
+  - intros x H1 H2.
+    unfold memory in *.
+    congruence.
+Qed.
+
+
+Lemma alter_singleton f l old :
+  alter f l ({[ l := old ]} : memory) = ({[l := f old ]} : memory).
+Proof using Type.
+  unfold memory in *.
+  now rewrite (alter_singleton_eq).
+Qed.
